proof/DDC/Language/SystemF2Data/TyJudge.v
@@ -1,0 +1,236 @@
+
+Require Export DDC.Language.SystemF2.Ki.
+Require Export DDC.Language.SystemF2.KiJudge.
+Require Export DDC.Language.SystemF2.TyEnv.
+Require Export DDC.Language.SystemF2Data.Def.
+Require Export DDC.Language.SystemF2Data.Exp.
+
+
+(* Type Judgement assigns a type to an expression. *)
+(* TODO: Allow data constructors to have polymorphics types *)
+Inductive TYPE (ds: defs) (ke: kienv) (te: tyenv) : exp -> ty -> Prop :=
+ (* Variables *)
+ | TYVar 
+   :  forall i t
+   ,  get i te = Some t
+   -> TYPE ds ke te (XVar i) t
+
+ (* Type abstraction *)
+ | TYLAM 
+   :  forall x1 t1
+   ,  TYPE ds (ke :> KStar) (liftTE 0 te) x1 t1 
+   -> TYPE ds ke             te           (XLAM x1) (TForall t1)
+
+ (* Type application *)
+ | TYAPP
+   :  forall x1 t1 t2
+   ,  TYPE ds ke te x1 (TForall t1)
+   -> KIND ke t2 KStar
+   -> TYPE ds ke te (XAPP x1 t2) (substTT 0 t2 t1)
+
+ (* Function abstraction *)
+ | TYLam
+   :  forall x t1 t2
+   ,  KIND ke t1 KStar
+   -> TYPE ds ke (te :> t1) x            t2
+   -> TYPE ds ke te         (XLam t1 x) (tFun t1 t2)
+
+ (* Applications *)
+ | TYApp
+   :  forall x1 x2 t1 t2
+   ,  TYPE ds ke te x1           (tFun t1 t2)
+   -> TYPE ds ke te x2           t1
+   -> TYPE ds ke te (XApp x1 x2) t2
+
+ (* Data Constructors *)
+ | TYCon 
+   :  forall xs dc dcs tsArgs tc
+   ,  getDataDef dc ds = Some (DefData     dc tsArgs (TCon tc))
+   -> getTypeDef tc ds = Some (DefDataType tc dcs)
+   -> In dc dcs
+   -> Forall2 (TYPE ds ke te) xs tsArgs
+   -> TYPE ds ke te (XCon dc xs) (TCon tc)
+
+ (* Case Expressions *)
+ | TYCase
+   :  forall xObj tcPat tResult alts dcs
+
+      (* check types of expression and alternatives *)
+   ,  TYPE ds ke te xObj (TCon tcPat)            
+   -> Forall (fun alt => TYPEA ds ke te alt (TCon tcPat) tResult) alts
+
+      (* there must be at least one alternative *)
+   -> length alts > 0
+
+      (* all data cons must have a corresponding alternative *)
+   -> getTypeDef tcPat ds = Some (DefDataType tcPat dcs)
+   -> Forall (fun dc => In dc (map dcOfAlt alts)) dcs
+
+   -> TYPE ds ke te (XCase xObj alts) tResult
+
+with TYPEA  (ds: defs) (ke: kienv) (te: tyenv) : alt -> ty -> ty -> Prop :=
+ (* Case Alternatives *)
+ | TYAlt 
+   :  forall x1 t1 dc tsArgs tResult
+   ,  getDataDef dc ds = Some (DefData dc tsArgs tResult)
+   -> TYPE  ds ke (te >< tsArgs) x1 t1
+   -> TYPEA ds ke te (AAlt dc tsArgs x1) tResult t1.
+
+Hint Constructors TYPE.
+Hint Constructors TYPEA.
+
+
+(* Invert all hypothesis that are compound typing statements. *)
+Ltac inverts_type :=
+ repeat 
+  (match goal with 
+   | [ H: TYPE  _ _ _ (XVar  _)    _    |- _ ] => inverts H
+   | [ H: TYPE  _ _ _ (XLAM  _)    _    |- _ ] => inverts H
+   | [ H: TYPE  _ _ _ (XAPP  _ _)  _    |- _ ] => inverts H
+   | [ H: TYPE  _ _ _ (XLam  _ _)  _    |- _ ] => inverts H
+   | [ H: TYPE  _ _ _ (XApp  _ _)  _    |- _ ] => inverts H
+   | [ H: TYPE  _ _ _ (XCon  _ _)  _    |- _ ] => inverts H
+   | [ H: TYPE  _ _ _ (XCase _ _)  _    |- _ ] => inverts H
+   | [ H: TYPEA _ _ _ (AAlt _ _ _) _ _  |- _ ] => inverts H
+   end).
+
+
+(********************************************************************)
+(* Forms of values. 
+   If we know the type of a value,
+   then we know the form of that value. *)
+Lemma value_lam 
+ :  forall x ds ke te t1 t2
+ ,  value x 
+ -> TYPE ds ke te x (tFun t1 t2)
+ -> (exists t x', x = XLam t x').
+Proof.
+ intros. destruct x; eauto; nope.
+Qed.
+Hint Resolve value_lam.
+
+
+(********************************************************************)
+(* A well typed expression is well formed *)
+Theorem type_wfX
+ :  forall ds ke te x t
+ ,  TYPE ds ke te x t
+ -> wfX ke te x.
+Proof.
+ intros. gen ds ke te t.
+ induction x using exp_mutind with 
+  (PA := fun a => forall ds ke te t1 t2
+      ,  TYPEA ds ke te a t1 t2 
+      -> wfA ke te a)
+  ; intros; inverts_type; eauto.
+
+ Case "XCon".
+  apply WfX_XCon.
+  nforall. intros.
+  eapply Forall2_exists_left in H7; eauto.
+  dest y. eauto.
+
+ Case "XCase".
+  eapply WfX_XCase.
+   eapply IHx. eauto.
+   nforall. eauto.
+Qed.
+Hint Resolve type_wfX.
+
+
+(* Weakening Type Env in Type Judgement.
+   We can insert a new type into the type environment, provided we
+   lift existing references to types higher in the stack across
+   the new one. *)
+Lemma type_tyenv_insert
+ :  forall ds ke te ix x t1 t2
+ ,  TYPE ds ke te x t1
+ -> TYPE ds ke (insert ix t2 te) (liftXX 1 ix x) t1.
+Proof.
+ intros. gen ix ds ke te t1 t2.
+ induction x using exp_mutind with 
+  (PA := fun a => forall ix ds ke te t2 t3 t4
+      ,  TYPEA ds ke te a t3 t4 
+      -> TYPEA ds ke (insert ix t2 te) (liftXA 1 ix a) t3 t4)
+  ; intros; inverts_type; simpl; eauto.
+
+ Case "XVar".
+  nnat. 
+  lift_cases; intros; auto.
+
+ Case "XLAM".
+  apply TYLAM.
+  assert ( liftTE 0 (insert ix t2 te)
+         = insert ix (liftTT 0 t2) (liftTE 0 te)).
+   unfold liftTE. rewrite map_insert. auto.
+   rewrite H. eauto.
+
+ Case "XLam".
+  apply TYLam; eauto.
+  rewrite insert_rewind. auto.
+
+ Case "XCon".
+  eapply TYCon; eauto.
+   nforall.
+   apply (Forall2_map_left (TYPE ds ke (insert ix t2 te))).
+   apply (Forall2_impl_in  (TYPE ds ke te)); eauto.
+
+ Case "XCase".
+  eapply TYCase; eauto.
+   apply Forall_map.
+   apply (Forall_impl_in 
+     (fun a => TYPEA ds ke te a (TCon tcPat) t1)); eauto.
+   nforall. eauto.
+
+  rewrite map_length; auto.
+
+  nforall.
+   intros. rename x0 into d. 
+   rewrite map_map. unfold compose.
+   eapply map_exists_in.
+   assert (In d (map dcOfAlt aa)). 
+    eauto.
+   assert (exists a, dcOfAlt a = d /\ In a aa).
+    eapply map_in_exists. auto.
+   shift a. subst. int. rewrite <- H7.
+   eapply dcOfAlt_liftXA.
+
+ Case "XAlt".
+  eapply TYAlt; eauto.
+  rewrite insert_app. auto.
+Qed. 
+
+
+(* We can push a new type onto the environment stack provided
+   we lift references to existing types across the new one. *)
+Lemma type_tyenv_weaken1
+ :  forall ds ke te x t1 t2
+ ,  TYPE ds ke te x t1
+ -> TYPE ds ke (te :> t2) (liftXX 1 0 x) t1.
+Proof.
+ intros.
+ assert (te :> t2 = insert 0 t2 te).
+  simpl. destruct te; auto.
+ rewrite H0.
+  apply type_tyenv_insert. auto.
+Qed.
+
+
+(* We can several new types onto the environment stack provided
+   we lift referenes to existing types across the new one. *)
+Lemma type_tyenv_weaken_append
+ :  forall ds ke te te' x t1
+ ,  TYPE ds ke te x t1
+ -> TYPE ds ke (te >< te') (liftXX (length te') 0 x) t1.
+Proof.
+ intros.
+ induction te'; simpl.
+  rewrite liftXX_zero. 
+   auto. 
+  rewrite <- nat_plus_one.
+   assert (length te' + 1 = 1 + length te') as HL. 
+    burn. rewrite HL. clear HL.
+   rewrite <- liftXX_plus.
+   eapply type_tyenv_weaken1. auto. 
+Qed.
+
